theories/typing/uniq_bor.v
@@ -42,7 +42,7 @@ Section uniq_bor.
   Qed.
 
   Global Instance uniq_bor_wf κ ty `{!TyWf ty} : TyWf (uniq_bor κ ty) :=
-    { ty_lfts := [κ]; ty_wf_E := ty.(ty_wf_E) ++ ty_outlives_E ty κ }.
+    { ty_lfts := [κ]; ty_wf_E := ty_wf_E ty ++ ty_outlives_E ty κ }.
 
   Lemma uniq_type_incl κ1 κ2 ty1 ty2 :
     κ2 ⊑ κ1 -∗
